Refactor list to use total functions

common.v
@@ -1,48 +1,62 @@
-From WR Require Import syntax typing.
-From Coq Require Import ssreflect.
+From WR Require Import syntax.
+From Coq Require Import ssreflect List.
 Require Import Psatz.
 From Hammer Require Import Tactics.
+Import ListNotations.
+
+Definition context := list tm.
+
+Fixpoint dep_ith Γ i :=
+  match Γ , i with
+  | (A :: Γ), 0 => ren_tm shift A
+  | (A :: Γ), (S i) => ren_tm shift (dep_ith Γ i)
+  | _, _ => tFalse
+  end.
+
+Notation ith Γ i := (nth i Γ tFalse).
+
+Lemma dep_ith_ren_tm (Γ : context) (A : tm) (x : fin) :
+  dep_ith (A :: Γ) (S x) = ren_tm shift (dep_ith Γ x).
+Proof. done. Qed.
+
+Lemma dep_ith_ren_tm0 (Γ : context) (A : tm) :
+  dep_ith (A :: Γ) 0 = ren_tm shift A.
+Proof. done. Qed.
 
 Definition good_renaming ξ Γ Δ :=
-  forall i A, dep_ith Γ i = Some A ->
-          dep_ith Δ (ξ i) = Some (ren_tm ξ A).
+  forall i, i < length Γ -> ξ i < length Δ /\ dep_ith Δ (ξ i) = ren_tm ξ (dep_ith Γ i).
 
+Lemma dep_ith_shift Γ i :
+  dep_ith Γ i = ren_tm (Nat.add (S i)) (ith Γ i).
+Proof.
+  elim : Γ i.
+  - hauto q:on.
+  - move => A Γ h.
+    case => [|i].
+    + done.
+    + simpl.
+      rewrite h.
+      by asimpl.
+Qed.
 
-Lemma nth_error_skipn {T : Type} n i Γ (A : T) :
-  nth_error (skipn n Γ) i = Some A ->
-  nth_error Γ (n + i) = Some A.
-  move : n i A.
+Lemma ith_skipn n i (Γ : context) :
+  ith (skipn n Γ) i = ith Γ (n + i).
+  move : n i.
   elim : Γ.
-  - hauto lq:on rew:off inv:nat ctrs:option.
-  - hauto lq:on rew:off inv:nat ctrs:option.
+  - hauto lq:on inv:nat.
+  - move => A Γ ih n i.
+    case : i; qauto l:on inv:nat.
 Qed.
 
 Lemma good_renaming_truncate n Γ :
   good_renaming (Nat.add n) (skipn n Γ) Γ .
 Proof.
-  rewrite /good_renaming => i A h.
-  rewrite dep_ith_shift_n in h.
-  remember (nth_error (skipn n Γ) i) as A0 eqn:eq.
-  case : A0 eq h => // A0 eq h.
-  apply eq_sym in eq.
-  apply nth_error_skipn in eq.
-  simpl in h.
-  case : h => * /=; subst.
-  rewrite dep_ith_shift_n.
-  rewrite eq => /=.
-  asimpl.
-  f_equal.
-  f_equal.
-  simpl.
-  rewrite /funcomp.
-  fext. lia.
+  rewrite /good_renaming => i h /=.
+  repeat rewrite dep_ith_shift.
+  rewrite ith_skipn.
+  split.
+  - rewrite skipn_length in h.
+    lia.
+  - asimpl. f_equal.
+    fext => ?; asimpl; lia.
 Qed.
-
-(* Lemma good_renaming_truncate' n m Γ : *)
-(*   n <= m -> *)
-(*   good_renaming (Nat.add n) (m - n) (Nat.add n >> Γ) m Γ. *)
-(* Proof. *)
-(*   move => h. *)
-(*   replace m with (n + (m - n)) at 2; last by lia. *)
-(*   apply good_renaming_truncate. *)
-(* Qed. *)
